Update heap.v w.r.t. iris recommandations
Update heap.v to make sure we can initialize the iris state
and build closed proofs.

theories/heap.v
@@ -5,18 +5,35 @@
  * LICENSE file in the root directory of this source tree.
  *)
 From stdpp Require Import strings.
-From iris.base_logic.lib Require Import iprop own.
+From iris.base_logic.lib Require Import iprop own ghost_map.
 From iris.algebra Require Import ofe cmra gmap_view.
 
 From shack Require Import lang.
 
 Canonical Structure tagO : ofe := leibnizO tag.
 Canonical Structure lang_tyO : ofe := leibnizO lang_ty.
+Canonical Structure valueO : ofe := leibnizO value.
 
 
 (* interpretation of types *)
 Definition sem_typeO (Σ : gFunctors) : ofe := value -d> iPropO Σ.
 
-Class sem_heapG (Σ : gFunctors) : Set := SemHeapG {
-  sem_heapG_heap :> inG Σ (gmap_viewR loc (prodO tagO (gmapO string (laterO (sem_typeO Σ)))));
+Definition sem_typeOF (F: oFunctor) : oFunctor :=
+  discrete_funOF (λ (_:value), F).
+
+Class sem_heapGpreS (Σ : gFunctors) : Set := {
+  sem_heap :> inG Σ (gmap_viewR loc (prodO tagO (gmapO string (laterO (sem_typeO Σ)))));
 }.
+
+Definition sem_heapΣ : gFunctors :=
+  #[GFunctor (gmap_viewRF loc (tagO * (gmapOF string (laterOF (sem_typeOF ∙)))))].
+
+Global Instance subG_sem_heapΣ {Σ}: subG sem_heapΣ Σ → sem_heapGpreS Σ.
+Proof.  solve_inG. Qed.
+
+Class sem_heapGS (Σ: gFunctors) := SemHeapGS {
+  sem_heap_inG :> sem_heapGpreS Σ;
+  sem_heap_name: gname;
+}.
+
+(* Lemma sem_heap_init `{!sem_heapGpreS Σ}: ⊢ |==> ∃ _ : sem_heapGS Σ, True%I. *)
